all files adjusted with mathlib styling

Future/Certification.lean
@@ -1,16 +1,21 @@
+/-
+Copyright (c) 2022 Tomaz Gomes. All rights reserved.
+Released under Apache 2.0 license as described in the file LICENSE.
+Author: Tomaz Gomes.
+-/
 import data.bool
 import data.list
-import MergeSortDirect
-import InsertionSortDirect
+import MergeSort.MergeSort
+import InsertionSort
 
-namespace counting
+namespace Timed
 
 variables {α : Type} (r : α → α → Prop) [decidable_rel r]
 local infix ` ≼ ` : 50 := r
 
 @[simp] def comparisons_insert (a : α) : list α → ℕ
 | [] := 0
-| (h :: t) := if a ≼ h then 0 else 1 + comparisons_insert t
+| (h :: t) := if a ≼ h then 1 else 1 + comparisons_insert t
 
 #eval comparisons_insert (λ m n : ℕ , m ≤ n) 6 [1, 3, 4, 9]
 -- 3
@@ -18,10 +23,9 @@ local infix ` ≼ ` : 50 := r
 #eval comparisons_insert (λ m n : ℕ , m ≤ n) 5 [0, 2, 3, 6]
 -- 3
 
-def remove_prefix (a : α) : list α → list α
+@[simp] def remove_prefix (a : α) : list α → list α
 | [] := []
-| (h :: t) := if a ≼ h
-              then h :: t
+| (h :: t) := if a ≼ h then h :: t
               else remove_prefix t
 
 #eval remove_prefix (λ m n : ℕ , m ≤ n) 2 [1, 2, 3, 4]
@@ -34,7 +38,13 @@ def remove_prefix (a : α) : list α → list α
 | []        ys        := 0
 | xs        []        := 0
 | (x :: xs) (y :: ys) := comparisons_insert r x (y :: ys) +
-                         comparisons_merge xs (remove_prefix r x)
+                         comparisons_merge xs (remove_prefix r x ys)
+
+def l₁ : list ℕ := [8, 1, 3]
+def l₂ : list ℕ := [14, 5, 6]
+
+#eval comparisons_merge (λ m n : ℕ, m ≤ n) l₁ l₂
+#eval prod.snd (merge (λ m n : ℕ, m ≤ n) l₁ l₂)
 
 theorem comparisons_insert_correct (a : α) : ∀ l : list α,
   (ordered_insert r a l).snd = comparisons_insert r a l :=
@@ -47,26 +57,31 @@ begin
     { rw ← l_ih,
       cases (ordered_insert r a l_tl),
       unfold ordered_insert,
+      rw add_comm,
     }
   }
 end
 
+
 theorem comparisons_merge_correct : ∀ l₁ l₂ : list α,
   (merge r l₁ l₂).snd = comparisons_merge r l₁ l₂
-| []         []         := begin simp, unfold merge, end
-| []         (h₂ :: t₂) := begin simp, unfold merge, end
-| (h₁ :: t₁) []         := begin simp, unfold merge, end
+| []         []         := begin simp only [comparisons_merge], unfold merge, end
+| []         (h₂ :: t₂) := begin simp only [comparisons_merge], unfold merge, end
+| (h₁ :: t₁) []         := begin simp only [comparisons_merge], unfold merge, end
 | (h₁ :: t₁) (h₂ :: t₂) :=
 begin
-  simp,
-  unfold remove_prefix,
-  unfold merge,
+  simp only [comparisons_insert, comparisons_merge, remove_prefix, merge],
   split_ifs,
   { have ih := comparisons_merge_correct t₁ (h₂ :: t₂),
-    cases (merge r t₁ (h₂ :: t₂)),
+    cases (merge r t₁ (h₂ :: t₂)) with _ cnt,
+
     unfold merge,
     simp at *,
-    rw ih,
+    
+    cases t₂,
+
+    { simp, rw ih, simp, },
+    rw ← ih,
     ring,
   },
   have ih := comparisons_merge_correct (h₁ :: t₁) t₂,
@@ -80,4 +95,4 @@ begin
 end
 
 
-end counting
+end Timed
