src/MergeSort/MergeSort.lean
@@ -1,240 +1,57 @@
+/-
+Copyright (c) 2022 Tomaz Gomes. All rights reserved.
+Released under Apache 2.0 license as described in the file LICENSE.
+Author: Tomaz Gomes.
+-/
 import data.list.sort tactic
 import data.nat.log
 import init.data.nat
 
-import MergeSort.Lemmas
+import MergeSort.LogLemmas
+import MergeSort.Split
+import MergeSort.Merge
+/-
+# Timed Merge Sort
+  This file defines a new version of Merge Sort that, besides sorting the input list, counts the
+  number of operations made through the execution of the algorithm. Also, it presents proofs of
+  it's time complexity and it's equivalence to the one defined in data/list/sort.lean
+## Main Definition:
+  - Timed.merge_sort : list α → (list α × ℕ)
+## Main Results:
+  - Timed.merge_sort_complexity :
+      ∀ l : list α, (Timed.merge_sort r l).snd ≤ 8 * l.length * nat.log 2 l.length
+  - Timed.merge_sort_equivalence :
+      ∀ l : list α, (Timed.merge_sort r l).fst = list.merge_sort r l
+     
+-/
 
 variables {α : Type} (r : α → α → Prop) [decidable_rel r]
 local infix ` ≼ ` : 50 := r
 
 namespace Timed
 
-@[simp] def split : list α → (list α × list α × ℕ)
-| []       := ([], [], 0)
-| (h :: t) := let (l₁, l₂, n) := split t in (h :: l₂, l₁, n + 1)
-
-theorem split_equivalence : ∀ (l : list α) ,
-  (split l).fst = (list.split l).fst ∧ (split l).snd.fst = (list.split l).snd
-| [] := by simp
-| (h :: t) :=
-begin
-  simp only [list.split, split],
-
-  have ih := split_equivalence t,
-  cases ih with ih_fst ih_snd,
-
-  cases (split t) with t_left₁ t_right₁,
-  cases t_right₁ with t_right₁ _,
-  unfold split,
-
-  cases t.split with t_left₂ t_right₂,
-  unfold list.split,
-  simp only [true_and, eq_self_iff_true],
-
-  exact ⟨ ih_snd, ih_fst ⟩,
-end
-
-theorem split_complexity : ∀ (l : list α) , (split l).snd.snd = l.length
-| [] := by simp
-| (h :: t) :=
-begin
-  simp only [list.length, split],
-  have IH := split_complexity t,
-  cases split t with l₁ l₂n,
-  cases l₂n with l₂ n,
-  unfold split,
-  rw add_left_inj,
-  exact IH,
-end
-
-theorem length_split_lt {a b: α} {l l₁ l₂ : list α} {n : ℕ}
-  (h : split (a::b::l) = (l₁, l₂, n)):
-    list.length l₁ < list.length (a::b::l) ∧
-    list.length l₂ < list.length (a::b::l) :=
-begin
-  have split_eq_full : l₁ = (a::b::l).split.fst ∧ l₂ = (a::b::l).split.snd :=
-  begin
-    have l₂_n_id : (l₂, n) = (split (a :: b :: l)).snd :=
-      (congr_arg prod.snd h).congr_right.mpr rfl,
-
-    have l₂_id : l₂ = (split (a :: b :: l)).snd.fst :=
-      (congr_arg prod.fst l₂_n_id).congr_right.mp rfl,
-
-    have l₁_id : l₁ = (split (a :: b :: l)).fst :=
-      (congr_arg prod.fst h).congr_right.mpr rfl,
-
-    have split_eq := split_equivalence (a :: b :: l),
-    cases split_eq,
-
-    rw split_eq_left at l₁_id,
-    rw split_eq_right at l₂_id,
-
-    exact ⟨ l₁_id , l₂_id ⟩,
-  end,
-  cases split_eq_full,
-  have reconstruct : (a::b::l).split = (l₁, l₂) :=
-  begin
-    rw split_eq_full_left,
-    rw split_eq_full_right,
-    exact prod.ext rfl rfl,
-  end ,
-  exact list.length_split_lt reconstruct,
-end
-
-theorem split_halves_length : ∀ {l l₁ l₂ : list α} {n : ℕ},
-  split l = (l₁, l₂, n) → 
-    2 * list.length l₁ ≤ list.length l + 1 ∧ 2 * list.length l₂ ≤ list.length l
-| []       :=
-begin
-  intros l₁ l₂ n h,
-  unfold split at h,
-  simp only [prod.mk.inj_iff] at h,
-  cases h  with h₁ h₂,
-  cases h₂ with h₂ _,
-  rw [← h₁, ← h₂],
-  simp,
-end
-| (h :: t) :=
-begin
-  intros l₁ l₂ n h',
-  cases e : split t with t₁ t₂m,
-  cases t₂m with t₂ m,
-
-  have split_id : split (h :: t) = (h :: t₂, t₁, m + 1) :=
-  begin
-    rw split,
-    cases split t with t₁' t₂',
-    cases t₂' with t₂' m₂,
-    unfold split,
-    injection e,
-    injection h_2,
-    refine congr (congr_arg prod.mk (congr_arg (list.cons h) h_3)) _,
-    rw h_1,
-    rw h_4,
-  end,
-  rw split_id at h',
-  injection h',
-  injection h_2,
-
-  have IH := split_halves_length e,
-  refine and.intro _ _,
-  { rw ← h_1, simp only [list.length], linarith, },
-  { rw ← h_3, simp only [list.length], linarith, },
-end
-
 include r
 
-theorem split_lengths : ∀ (l l₁ l₂ : list α) {n : ℕ},
-  split l = (l₁, l₂, n) → l₁.length + l₂.length = l.length
-| []  := by { intros l₁ l₂ n,
-              simp only [and_imp, prod.mk.inj_iff, list.length, add_eq_zero_iff, split],
-              intros h₁ h₂ _,
-              rw [← h₁, ← h₂],
-              simp,
-            }
-| [a] := by { intros l₁ l₂ n,
-              simp only [and_imp, prod.mk.inj_iff, list.length_singleton, zero_add, split],
-              intros h₁ h₂ _,
-              rw [← h₁, ← h₂],
-              simp,
-            }
-| (a :: b :: t) :=
-begin
-  intros l₁ l₂ n h,
-  cases e : split t with l₁' l₂'m,
-  cases l₂'m with l₂' m,
-  simp only [split] at h,
-  rw e at h,
-  unfold split at h,
-  have ih := split_lengths t l₁' l₂' e,
-  injection h,
-  injection h_2,
-  rw [← h_1, ← h_3],
-  simp only [list.length], linarith,
-end
-
-def merge : list α → list α → (list α × ℕ)
-| []       l'        := (l', 0)
-| l        []        := (l,  0)
-| (a :: l) (b :: l') := if a ≼ b
-                        then let (l'', n) :=
-                                   merge l (b :: l') in (a :: l'', n + 1)
-                        else let (l'', n) :=
-                                   merge (a :: l) l' in (b :: l'', n + 1)
-
-theorem merge_complexity : ∀ l l' : list α,
-  (merge r l l').snd ≤ l.length + l'.length
-| []   []               := by { unfold merge, simp }
-| []   (h' :: t')       := by { unfold merge, simp }
-| (h :: t)    []        := by { unfold merge, simp }
-| (h₁ :: t₁) (h₂ :: t₂) :=
-begin
-  unfold merge, split_ifs,
-  { have IH := merge_complexity t₁ (h₂ :: t₂),
-    cases (merge r t₁ (h₂ :: t₂)),
-    unfold merge,
-    simp only [list.length] at IH,
-    simp only [list.length],
-    linarith,
-  },
-  { have IH := merge_complexity (h₁ :: t₁) t₂,
-    cases (merge r (h₁ :: t₁) t₂),
-    unfold merge,
-    simp only [list.length] at IH,
-    simp only [list.length],
-    linarith,
-  }
-end
-
-theorem merge_equivalence : ∀ l l' : list α,
-  (merge r l l').fst = list.merge r l l'
-| []       []         := by { unfold merge, unfold list.merge }
-| []       (h' :: t') := by { unfold merge, unfold list.merge }
-| (h :: t) []         := by { unfold merge, unfold list.merge }
-| (h :: t) (h' :: t') :=
-begin
-  unfold merge,
-  split_ifs,
-  { have ih := merge_equivalence t (h' :: t'),
-    cases (merge r t (h' :: t')),
-    unfold merge,
-
-    unfold list.merge,
-    split_ifs,
-    exact ⟨ rfl, ih ⟩,
-  },
-  { have ih := merge_equivalence (h :: t) t',
-    cases (merge r (h :: t) t'),
-    unfold merge,
-
-    unfold list.merge,
-    split_ifs,
-    exact ⟨ rfl, ih ⟩,
-  }
-end
-
--- MERGE SORT DEFINITIONS
-
 def merge_sort : list α → (list α × ℕ)
-| []        := ([],  0)
-| [a]       := ([a], 0)
-| (a::b::l) := begin
-  cases e : split (a::b::l) with l₁ l₂n,
+| []            := ([],  0)
+| [a]           := ([a], 0)
+| (a :: b :: l) := begin
+  cases e : split (a :: b :: l) with l₁ l₂n,
   cases l₂n with l₂ n,
   cases length_split_lt e with h₁ h₂,
   have ms₁ := merge_sort l₁,
   have ms₂ := merge_sort l₂,
   have merged := merge r ms₁.fst ms₂.fst,
-  have split_ops := (split (a::b::l)).snd.snd,
-  exact ( merged.fst , split_ops + ms₁.snd + ms₂.snd + merged.snd),
+  have split_ops := (split (a :: b :: l)).snd.snd,
+  exact (merged.fst , split_ops + ms₁.snd + ms₂.snd + merged.snd),
 end
 using_well_founded {
   rel_tac := λ_ _, `[exact ⟨_, inv_image.wf list.length nat.lt_wf⟩],
   dec_tac := tactic.assumption }
 
 theorem merge_sort_cons_cons_fst {a b n} {l l₁ l₂ : list α}
-  (h : split (a::b::l) = (l₁, l₂, n)) :
-  (merge_sort r (a::b::l)).fst = (merge r (merge_sort r l₁).fst (merge_sort r l₂).fst).fst :=
+  (h : split (a :: b :: l) = (l₁, l₂, n)) :
+  (merge_sort r (a :: b :: l)).fst = (merge r (merge_sort r l₁).fst (merge_sort r l₂).fst).fst :=
 begin
   suffices : ∀ (L : list α × ℕ) h1, (@@and.rec
     (λ a a (_ : list.length l₁ < list.length l + 1 + 1 ∧
@@ -247,20 +64,20 @@ theorem merge_sort_equivalence : ∀ l : list α , (merge_sort r l).fst = list.m
 | []       := by { unfold merge_sort, unfold list.merge_sort }
 | [a]      := by { unfold merge_sort, unfold list.merge_sort }
 | (a₁ :: a₂ :: t) :=
-have (split (a₁ :: a₂ :: t)).fst.length < (a₁ :: a₂ :: t).length :=
-begin
-  cases e : split (a₁ :: a₂ :: t) with l₁ l₂n,
-  cases l₂n with l₂ n,
-  cases length_split_lt e with h₁ h₂,
-  exact h₁,
-end,
-have (split (a₁ :: a₂ :: t)).snd.fst.length < (a₁ :: a₂ :: t).length :=
-begin
-  cases e : split (a₁ :: a₂ :: t) with l₁ l₂n,
-  cases l₂n with l₂ n,
-  cases length_split_lt e with h₁ h₂,
-  exact h₂,
-end,
+  have (split (a₁ :: a₂ :: t)).fst.length < (a₁ :: a₂ :: t).length :=
+  begin
+    cases e : split (a₁ :: a₂ :: t) with l₁ l₂n,
+    cases l₂n with l₂ n,
+    cases length_split_lt e with h₁ h₂,
+    exact h₁,
+  end,
+  have (split (a₁ :: a₂ :: t)).snd.fst.length < (a₁ :: a₂ :: t).length :=
+  begin
+    cases e : split (a₁ :: a₂ :: t) with l₁ l₂n,
+    cases l₂n with l₂ n,
+    cases length_split_lt e with h₁ h₂,
+    exact h₂,
+  end,
 begin
   rw list.merge_sort_cons_cons r (prod.ext rfl rfl),
   rw merge_sort_cons_cons_fst r (prod.ext rfl (prod.ext rfl rfl)),
@@ -273,13 +90,12 @@ end
 using_well_founded {rel_tac := λ _ _, `[exact ⟨_, measure_wf list.length⟩]}
 
 theorem merge_sort_cons_cons_snd {a b n} {l l₁ l₂ : list α}
-  (hs : split (a::b::l) = (l₁, l₂, n)) :
-  (merge_sort r (a::b::l)).snd =
-    (split (a::b::l)).snd.snd +
+  (hs : split (a :: b :: l) = (l₁, l₂, n)) :
+  (merge_sort r (a :: b :: l)).snd =
+    (split (a :: b :: l)).snd.snd +
     (merge_sort r l₁).snd +
     (merge_sort r l₂).snd +
-    (merge r (merge_sort r l₁).fst (merge_sort r l₂).fst).snd
-  :=
+    (merge r (merge_sort r l₁).fst (merge_sort r l₂).fst).snd :=
 begin
   suffices : ∀ (L : list α × ℕ) h1, (@@and.rec
     (λ a a (_ : list.length l₁ < list.length l + 1 + 1 ∧
@@ -288,33 +104,27 @@ begin
   intros, cases h1, refl,
 end
 
-
 theorem merge_sort_complexity : ∀ l : list α,
   (merge_sort r l).snd ≤ 8 * l.length * nat.log 2 l.length
-| []  := by { unfold merge_sort, simp }
-| [a] := by { unfold merge_sort, simp }
+| []  := by { unfold merge_sort, simp only [nat.log_zero_right, list.length, mul_zero] }
+| [a] := by { unfold merge_sort, simp only [nat.log_one_right, list.length_singleton, mul_zero] }
 | (a₁ :: a₂ :: t) :=
 let l := (a₁ :: a₂ :: t) in
 begin
   rw merge_sort_cons_cons_snd r (prod.ext rfl (prod.ext rfl rfl)),
   rw split_complexity,
-
   cases hs : split l with l₁ l₂n,
   cases l₂n with l₂ n,
-
-  cases length_split_lt hs with hh₁ hh₂,
-
   have l₁_length : 2 * l₁.length ≤ l.length + 1 := (split_halves_length hs).1,
   have l₂_length : 2 * l₂.length ≤ l.length     := (split_halves_length hs).2,
   have l₂_length_half : l₂.length ≤ l.length / 2 := div_two l.length l₂.length l₂_length,
   have ih₁ := merge_sort_complexity l₁,
   have ih₂ := merge_sort_complexity l₂,
-
-  cases h₁ : merge_sort r l₁ with l₁s ns,
-  cases h₂ : merge_sort r l₂ with l₂s ms,
-
   have t_len_l_len : t.length + 2 = l.length := rfl,
   have l₁_length_weak : l₁.length ≤ l.length := by linarith,
+  cases length_split_lt hs with hh₁ hh₂,
+  cases h₁ : merge_sort r l₁ with l₁s ns,
+  cases h₂ : merge_sort r l₂ with l₂s ms,
 
   have ms_bound : ms ≤ 4 * l.length * (nat.log 2 l.length - 1) :=
   begin
@@ -323,12 +133,20 @@ begin
     refine le_trans ih₂ _,
     rw log_pred l.length,
     calc 8 * l₂.length * nat.log 2 l₂.length
-                = 4 * (2 * l₂.length) * nat.log 2 l₂.length : by linarith
-            ... ≤ 4 * l.length * nat.log 2 l₂.length : begin rw mul_assoc, rw mul_assoc 4 l.length (nat.log 2 l₂.length),
-                                                             refine (mul_le_mul_left zero_lt_four).mpr _,
-                                                             exact nat.mul_le_mul_right (nat.log 2 l₂.length) l₂_length,
-                                                       end
-            ... ≤ 4 * l.length * nat.log 2 (l.length / 2) : begin refine nat.mul_le_mul_left (4 * l.length) _, exact log_monotonic l₂_length_half, end
+                = 4 * (2 * l₂.length) * nat.log 2 l₂.length :
+                      by linarith
+            ... ≤ 4 * l.length * nat.log 2 l₂.length :
+                      begin
+                        rw mul_assoc,
+                        rw mul_assoc 4 l.length (nat.log 2 l₂.length),
+                        refine (mul_le_mul_left zero_lt_four).mpr _,
+                        exact nat.mul_le_mul_right (nat.log 2 l₂.length) l₂_length,
+                      end
+            ... ≤ 4 * l.length * nat.log 2 (l.length / 2) :
+                      begin
+                        refine nat.mul_le_mul_left (4 * l.length) _,
+                        exact log_monotonic l₂.length (l.length / 2) l₂_length_half,
+                      end
   end,
 
   have ns_bound : ns ≤ 4 * (l.length + 1) * nat.log 2 l.length :=
@@ -337,12 +155,20 @@ begin
     rw ← ns_id,
     refine le_trans ih₁ _,
     calc 8 * l₁.length * nat.log 2 l₁.length
-                = 4 * (2 * l₁.length) * nat.log 2 l₁.length : by linarith
-            ... ≤ 4 * (l.length + 1) * nat.log 2 l₁.length : begin rw mul_assoc, rw mul_assoc 4 (l.length + 1) (nat.log 2 l₁.length),
-                                                                   refine (mul_le_mul_left zero_lt_four).mpr _,
-                                                                   exact nat.mul_le_mul_right (nat.log 2 l₁.length) l₁_length,
-                                                             end
-            ... ≤ 4 * (l.length + 1) * nat.log 2 l.length : begin refine nat.mul_le_mul_left (4 * (l.length + 1)) _, exact log_monotonic l₁_length_weak, end
+                = 4 * (2 * l₁.length) * nat.log 2 l₁.length :
+                      by linarith
+            ... ≤ 4 * (l.length + 1) * nat.log 2 l₁.length :
+                      begin
+                        rw mul_assoc,
+                        rw mul_assoc 4 (l.length + 1) (nat.log 2 l₁.length),
+                        refine (mul_le_mul_left zero_lt_four).mpr _,
+                        exact nat.mul_le_mul_right (nat.log 2 l₁.length) l₁_length,
+                      end
+            ... ≤ 4 * (l.length + 1) * nat.log 2 l.length :
+                      begin
+                        refine nat.mul_le_mul_left (4 * (l.length + 1)) _,
+                        exact log_monotonic l₁.length l.length l₁_length_weak,
+                      end
   end,
 
   have split_length : l₁s.length + l₂s.length = l.length :=
@@ -376,7 +202,10 @@ begin
   have log_l_length : 1 ≤ nat.log 2 l.length :=
   begin
     calc 1 = nat.log 2 2 : log_2_val.symm
-         ... ≤ nat.log 2 l.length : by { refine log_monotonic _, linarith, },
+         ... ≤ nat.log 2 l.length : begin
+                                      refine log_monotonic 2 l.length _,
+                                      linarith,
+                                    end
   end,
 
   have four_log_l_length : 4 * 1 * l.length ≤ 4 * nat.log 2 l.length * l.length :=
@@ -384,60 +213,67 @@ begin
     simp only [mul_le_mul_right, nat.succ_pos', mul_one, list.length],
     rw t_len_l_len,
     calc 4 = 4 * 1 : rfl
-         ... ≤ 4 * nat.log 2 l.length : by { refine mul_le_mul' _ log_l_length, exact le_refl 4, }
+         ... ≤ 4 * nat.log 2 l.length : begin
+                                          refine mul_le_mul' _ log_l_length,
+                                          exact le_refl 4,
+                                        end
   end,
 
   calc l.length + ns + ms + (merge r l₁s l₂s).snd
-           ≤ l.length + ns + ms + (l₁s.length + l₂s.length) : add_le_add_left (merge_complexity r l₁s l₂s) (l.length + ns + ms)
-      ...  = l.length + ns + ms + l.length : congr_arg (has_add.add (list.length l + ns + ms)) split_length
-      ...  = 2 * l.length + ns + ms : by ring
-      ...  ≤ 2 * l.length + ns + 4 * l.length * (nat.log 2 l.length - 1) : by { refine add_le_add_left _ (2 * l.length + ns), exact ms_bound, }
-      ...  ≤ 2 * l.length + 4 * l.length * (nat.log 2 l.length - 1) + ns : by ring_nf
-      ...  ≤ 2 * l.length + 4 * l.length * (nat.log 2 l.length - 1) + 4 * (l.length + 1) * nat.log 2 l.length :
-        begin
-          refine add_le_add_left _ (2 * l.length + 4 * l.length * (nat.log 2 l.length - 1)),
-          exact ns_bound,
-        end
-      ...  ≤ 8 * l.length * nat.log 2 (l.length) :
-        begin
-          ring_nf,
-          rw [ nat.mul_sub_left_distrib
-             , add_mul
-             , add_mul
-             , nat.mul_sub_right_distrib
-             ],
-          refine (add_le_add_iff_left (4 * 1 * l.length)).mp _,
-          rw [ ← add_assoc
-             , ← add_assoc
-             , ← add_assoc
-             , ← nat.add_sub_assoc four_log_l_length (4 * 1 * l.length)
-             , add_comm (4 * 1 * l.length) (4 * nat.log 2 l.length * l.length) 
-             , nat.add_sub_assoc rfl.ge (4 * nat.log 2 l.length * l.length)
-             , nat.sub_self (4 * 1 * l.length)
-             ],
-
-          simp only [add_zero, mul_one, list.length],
-          rw t_len_l_len,
-          ring_nf,
-
-          rw [ add_mul
-             , mul_assoc
-             , mul_comm l.length (nat.log 2 l.length)
-             , ← mul_assoc
-             , add_assoc
-             ],
-
-          refine (add_le_add_iff_left (8 * nat.log 2 l.length * l.length)).mpr _,
-          refine sum_2b (4 * nat.log 2 l.length) l.length _,
-
-          rw ← t_len_l_len,
-          have four_two_two: 4 = 2 * 2 := rfl,
-          rw four_two_two,
-          rw mul_assoc,
-          refine mul_le_mul' (le_refl 2) _,
-          
-          exact log_2_times t.length,
-        end,
+     ≤ l.length + ns + ms + (l₁s.length + l₂s.length) :
+          add_le_add_left (merge_complexity r l₁s l₂s) (l.length + ns + ms)
+ ... = l.length + ns + ms + l.length :
+          congr_arg (has_add.add (list.length l + ns + ms)) split_length
+ ... = 2 * l.length + ns + ms :
+          by ring
+ ... ≤ 2 * l.length + ns + 4 * l.length * (nat.log 2 l.length - 1) :
+          begin
+            refine add_le_add_left _ (2 * l.length + ns),
+            exact ms_bound,
+          end
+ ... ≤ 2 * l.length + 4 * l.length * (nat.log 2 l.length - 1) + ns :
+          by ring_nf
+ ... ≤ 2 * l.length + 4 * l.length * (nat.log 2 l.length - 1) + 4 * (l.length + 1) *
+       nat.log 2 l.length :
+          begin
+            refine add_le_add_left _ (2 * l.length + 4 * l.length * (nat.log 2 l.length - 1)),
+            exact ns_bound,
+          end
+ ... ≤ 8 * l.length * nat.log 2 l.length :
+          begin
+            ring_nf,
+            rw [ nat.mul_sub_left_distrib
+               , add_mul
+               , add_mul
+               , nat.mul_sub_right_distrib
+               ],
+            refine (add_le_add_iff_left (4 * 1 * l.length)).mp _,
+            rw [ ← add_assoc
+               , ← add_assoc
+               , ← add_assoc
+               , ← nat.add_sub_assoc four_log_l_length (4 * 1 * l.length)
+               , add_comm (4 * 1 * l.length) (4 * nat.log 2 l.length * l.length) 
+               , nat.add_sub_assoc rfl.ge (4 * nat.log 2 l.length * l.length)
+               , nat.sub_self (4 * 1 * l.length)
+               ],
+            simp only [add_zero, mul_one, list.length],
+            rw t_len_l_len,
+            ring_nf,
+            rw [ add_mul
+               , mul_assoc
+               , mul_comm l.length (nat.log 2 l.length)
+               , ← mul_assoc
+               , add_assoc
+               ],
+            refine (add_le_add_iff_left (8 * nat.log 2 l.length * l.length)).mpr _,
+            refine sum_2b (4 * nat.log 2 l.length) l.length _,
+            rw ← t_len_l_len,
+            have four_two_two: 4 = 2 * 2 := rfl,
+            rw four_two_two,
+            rw mul_assoc,
+            refine mul_le_mul' (le_refl 2) _,
+            exact log_2_times t.length,
+          end,
 end
 using_well_founded {rel_tac := λ _ _, `[exact ⟨_, measure_wf list.length⟩]}
 
